Adapting the proof to multiple calls to trapdoor test

examples/trapdoor.ec
@@ -1,19 +1,84 @@
-require import Prime_field.
-require import Cyclic_group_prime.
-require Int.
+require import Int.
 require import FSet.
 require import Bool.
 require import Real.
+require import AlgTactic.
+require import Prime_field.
+require import Cyclic_group_prime.
 
 import Dgroup.
 import Dgf_q.
 
-(* axioms *)
-axiom gen_exp_inj : forall(m n : gf_q), g ^ m = g ^ n => m = n.
-axiom neg_distr : forall (x y : gf_q), -(x + y) = -x + -y.
-axiom neg_zero : forall (x y : gf_q), gf_q0 = x - y => x = y.
+type zq = gf_q.
+
+op pow : zq -> int -> zq.
+op (^^) = pow.
+
+axiom qf_expr0 : forall (x : zq), x^^0 = gf_q1.
+axiom qf_exprS : forall (x : zq) i, 0 <= i => x^^(i+1) = x * x^^i.
+axiom qf_exprN : forall (x : zq) i, 0 <= i => x^^(-i) = inv (x^^i).
+
+
+op ofint : int -> zq.
+
+axiom qf_ofint0 : ofint 0 = Prime_field.gf_q0.
+axiom qf_ofint1 : ofint 1 = Prime_field.gf_q1.
+axiom qf_ofintS : forall i, 0 <= i => ofint (i+1) = ofint i + gf_q1.
+axiom qf_ofintN : forall (i : int), ofint (-i) = -(ofint i).
+
+instance field with zq
+  op rzero = Prime_field.gf_q0
+  op rone  = Prime_field.gf_q1
+  op add   = Prime_field.( + )
+  op opp   = Prime_field.([-])
+  op mul   = Prime_field.( * )
+  op expr  = pow
+  op sub   = Prime_field.( - )
+  op ofint = ofint
+  op inv   = Prime_field.inv
+  op div   = Prime_field.(/)
+
+  proof oner_neq0 by smt
+  proof addr0     by smt
+  proof addrA     by smt
+  proof addrC     by smt
+  proof addrN     by smt
+  proof mulr1     by smt
+  proof mulrA     by smt
+  proof mulrC     by smt
+  proof mulrDl    by smt
+  proof mulrV     by smt
+  proof expr0     by smt
+  proof exprS     by smt
+  proof exprN     by smt
+  proof subrE     by smt
+  proof divrE     by smt
+  proof ofint0    by smt
+  proof ofint1    by smt
+  proof ofintS    by smt
+  proof ofintN    by smt.
+
 
 (* lemmas of groups and prime field *)
+lemma gen_exp_inj : forall(m n : gf_q), g ^ m = g ^ n => m = n.
+proof.
+ intros => m n heq.
+ cut: log (g ^ m) = log (g ^n).
+  by rewrite heq.
+ by rewrite !group_pow_log.
+save.
+
+lemma neg_distr : forall (x y : gf_q), -(x + y) = -x + -y.
+proof.
+ by intros => ? ?; fieldeq.
+save.
+
+lemma neg_zero : forall (x y : gf_q), gf_q0 = x - y => x = y.
+proof.
+ intros => ? ? ?.
+ fieldeq; rewrite H; fieldeq.
+save.
+
 lemma gen_def : forall X, exists m, X = g ^ m. 
 proof.
  intros X; exists (log X).
@@ -242,417 +307,272 @@ proof.
  by rewrite -(group_log_pow X) H group_log_pow.
 save.
  
-(* given two group elements, pick 3 group elements Z1, Z2 and Y *)
-module type Pick = {
- fun pick (X1 : group, X2 : group) : group * group * group {*}
+
+const qO : int. (* bound on calls *)
+
+module type O = {
+ fun check (Z1 Z2 Y : group) : bool
+}.
+
+module type Adv (O : O) = {
+ fun run (X1 : group, X2 : group) : bool {* O.check}
+}.
+
+module M = {
+ var r, s : gf_q
+ var gx1, gx2 : group
+ var bad : bool
+ var cO : int
 }.
 
 
-module Trapdoor1( P : Pick) ={
+module Trapdoor1( A : Adv) ={
+  module TD : O ={
+   fun check (Z1 Z2 Y : group) : bool ={
+   var r : bool = false;
+   if (M.cO < qO){
+    r = (Z1 = Y ^(log M.gx1) /\ Z2 = Y ^(log M.gx2));
+   }
+   return r;
+   }
+ }
+ module AT = A(TD)
  fun main () : bool = {
-  var vX1, vZ1, vX2, vZ2, vY : group;
-  var r, s : gf_q;
-  vX1 = $dgroup;
-  r = $dgf_q; (* except gf_q0 *)
-  s = $dgf_q;
-  vX2 = (g ^ s) / (vX1 ^ r);
-  (vZ1, vZ2, vY) = P.pick(vX1, vX2);
-  return (vZ1 = vY ^(log vX1) /\ vZ2 = vY ^(log vX2));
+  var b : bool;
+  M.gx1 = $dgroup;
+  M.r = $dgf_q;
+  M.s = $dgf_q;
+  M.gx2 = (g ^ M.s) / (M.gx1 ^ M.r);
+  M.cO = 0;
+  b = AT.run(M.gx1, M.gx2);
+  return b;
  }
 }.
 
-
-module Trapdoor2( P : Pick) ={
+module Trapdoor2( A : Adv) ={
+ module TD : O = {
+  fun check (Z1 Z2 Y : group) : bool ={
+  var r : bool = false;
+  if (M.cO < qO){
+   r = ((Z1 ^ M.r) * Z2 = Y ^ M.s);
+   }
+  return r ;
+  }
+ }
+ module AT = A(TD)
  fun main () : bool = {
-  var vX1, vZ1, vX2, vZ2, vY : group;
-  var r, s : gf_q;
-  vX1 = $dgroup;
-  r = $dgf_q;
-  s = $dgf_q;
-  vX2 = (g ^ s) / (vX1 ^ r);
-  (vZ1, vZ2, vY) = P.pick(vX1, vX2);
-  return ((vZ1 ^ r) * vZ2 = vY^s);
+  var b : bool;
+  M.gx1 = $dgroup;
+  M.r = $dgf_q;
+  M.s = $dgf_q;
+  M.gx2 = (g ^ M.s) / (M.gx1 ^ M.r);
+  M.cO = 0;
+  b = AT.run(M.gx1, M.gx2);
+  return b;
  }
 }.
+
+(* module Trapdoor2( P : Pick) ={ *)
+(*  fun main () : bool = { *)
+(*   var vX1, vZ1, vX2, vZ2, vY : group; *)
+(*   var r, s : gf_q; *)
+(*   vX1 = $dgroup; *)
+(*   r = $dgf_q; *)
+(*   s = $dgf_q; *)
+(*   vX2 = (g ^ s) / (vX1 ^ r); *)
+(*   (vZ1, vZ2, vY) = P.pick(vX1, vX2); *)
+(*   return ((vZ1 ^ r) * vZ2 = vY^s); *)
+(*  } *)
+(* }. *)
 
 section.
 
-declare module P : Pick.
+declare module A : Adv {M}.
 
-axiom pick_ll : islossless P.pick.
+axiom run_ll : forall (O <: O{A}), islossless O.check => islossless A(O).run.
 
-local module G1 ( P : Pick) = {
- var bad : bool
- fun main () : bool = {
-  var vX1, vZ1, vX2, vZ2, vY : group;
-  var r, s : gf_q;
-  bad = false;
-  vX1 = $dgroup;
-  r = $dgf_q;
-  s = $dgf_q;
-  vX2 = (g ^ s) / (vX1 ^ r);
-  (vZ1, vZ2, vY) = P.pick(vX1, vX2);
-  if (vZ1 <> (vY^ (log vX1)) /\ ((vZ1 / (vY^ (log vX1))) ^r = (vY^(log vX2)) / vZ2)) {
-   bad = true;
+module G1( A : Adv) ={
+ module TD : O ={
+  fun check (Z1 Z2 Y : group) : bool ={
+  var r : bool = false;
+  if (M.cO < qO ){
+    r = (Z1 / (Y^ (log M.gx1))) ^ M.r = (Y^(log M.gx2)) / Z2;
+    if (Z1 <> (Y^ (log M.gx1)) /\ ((Z1 / (Y^ (log M.gx1))) ^ M.r = (Y^(log M.gx2)) / Z2)) {
+     M.bad = true;
+    }
+   }
+     return r;
   }
-  return ((vZ1 / (vY^ (log vX1))) ^r = (vY^(log vX2)) / vZ2);
+ }
+ module AT = A(TD)
+ fun main () : bool = {
+  var b : bool;
+  M.gx1 = $dgroup;
+  M.r = $dgf_q;
+  M.s = $dgf_q;
+  M.gx2 = (g ^ M.s) / (M.gx1 ^ M.r);
+  M.bad = false;
+  M.cO = 0;
+  b = AT.run(M.gx1, M.gx2);
+  return b;
  }
 }.
 
-
 local equiv Eq1 : 
-Trapdoor2(P).main ~ G1(P).main : true ==> ={res}.
+Trapdoor2(A).main ~ G1(A).main : true ==> ={res}.
 proof.
  fun.
- wp.
- call (_ : true); wp.
- do!rnd; wp.
- skip; progress => //.
- cut ->:= test_rewrite x1 x2 x3 rL sL (log vX1L) (log (g ^ sL / vX1L ^ rL)) _ => //. 
+ call (_ : ={M.gx1, M.gx2, M.r, M.s, M.cO} /\ (M.gx2 = g ^ M.s / M.gx1 ^ M.r){2}).
+ fun; wp; skip; progress.
+ cut ->:= test_rewrite Z1{2} Z2{2} Y{2} M.r{2} M.s{2} (log M.gx1{2}) (log (g ^ M.s{2} / M.gx1{2} ^ M.r{2})) _ => //. 
  rewrite log_div_minus.
  rewrite group_pow_log.
  by rewrite log_pow_mult /Prime_field.(-) gf_q_add_comm -gf_q_add_assoc 
- -(gf_q_add_comm (rL * log vX1L))  gf_q_add_minus gf_q_add_comm gf_q_add_unit.
+ -(gf_q_add_comm (M.r{2} * log M.gx1{2}))  gf_q_add_minus gf_q_add_comm gf_q_add_unit.
+ wp; do 3! rnd; skip; progress => //.
 save.
 
 local lemma Pr1 &m : 
-Pr [Trapdoor2(P).main() @ &m : res] =
-Pr [G1(P).main() @ &m : res]. 
+Pr [Trapdoor2(A).main() @ &m : res] =
+Pr [G1(A).main() @ &m : res]. 
 proof.
  equiv_deno Eq1 => //.
 save.
 
 local equiv Eq2 :
-Trapdoor1(P).main ~ G1(P).main : true ==> ! G1.bad{2} => ={res}.
+Trapdoor1(A).main ~ G1(A).main : true ==> ! M.bad{2} => ={res}.
 proof.
  fun.
- wp; call (_ : true).
- wp.
- do!rnd; wp.
- skip; progress => //.
- cut: (x1 = x3 ^ log vX1L /\ x2 = x3 ^ log (g ^ sL / vX1L ^ rL) <=>
-((x1 / x3 ^ log vX1L) ^ rL = x3 ^ log (g ^ sL / vX1L ^ rL) / x2)); last by smt.
+ call (_ : M.bad, 
+          ={M.gx1, M.gx2, M.r, M.s, M.cO} /\ (M.gx2 = g ^ M.s / M.gx1 ^ M.r){2}) => //.
+ apply run_ll. 
+ fun; wp; skip; progress => //.
+ cut: (Z1{2} = Y{2} ^ log M.gx1{2} /\ Z2{2} = Y{2} ^ log (g ^ M.s{2} / M.gx1{2} ^ M.r{2}) <=>
+((Z1{2} / Y{2} ^ log M.gx1{2}) ^ M.r{2} = Y{2} ^ log (g ^ M.s{2} / M.gx1{2} ^ M.r{2}) / Z2{2})); last by smt.
  split.
  intros => [heq1 heq2].
  rewrite heq1 heq2 /Cyclic_group_prime.(/) !gf_q_minus group_pow_mult.
  by rewrite gf_q_mult_comm gf_q_mult_zero.
  intros heq.
- cut :( x1 = x3 ^ log vX1L \/
-       ! (x1 / x3 ^ log vX1L) ^ rL = x3 ^ log (g ^ sL / vX1L ^ rL) / x2) by smt => {H8} H8.
+ cut :( Z1{2} = Y{2} ^ log M.gx1{2} \/
+       ! (Z1{2} / Y{2} ^ log M.gx1{2}) ^ M.r{2} = Y{2} ^ log (g ^ M.s{2} / M.gx1{2} ^ M.r{2}) / Z2{2}) by smt.
+ intros H8.
  elim H8 => heq'.
  split => //.
- cut:  (! x2 = x3 ^ log (g ^ sL / vX1L ^ rL) => false); last by smt.
+ cut:  (! Z2{2} = Y{2} ^ log (g ^ M.s{2} / M.gx1{2} ^ M.r{2}) => false); last by smt.
  intros => hneq; generalize heq => /=.
   rewrite heq' mult_div_I I_pow_n.
   rewrite div_eq_I.
  smt.
  smt.
+ by intros => ? h; fun; wp.
+ by intros => ?; fun; wp; skip.
+ wp; do 3! rnd; skip; progress; smt.
 save.
 
 local lemma Pr2_aux &m : 
-Pr [Trapdoor1(P).main() @ &m : res] <=
-Pr [G1(P).main() @ &m : res] + Pr[G1(P).main() @ &m : G1.bad]. 
+Pr [Trapdoor1(A).main() @ &m : res] <=
+Pr [G1(A).main() @ &m : res] + Pr[G1(A).main() @ &m : M.bad]. 
 proof.
- apply (Real.Trans _ (Pr [G1(P).main() @ &m : res \/ G1.bad]) _).
+ apply (Real.Trans _ (Pr [G1(A).main() @ &m : res \/ M.bad]) _).
  equiv_deno Eq2; smt.
  rewrite Pr mu_or; smt.
 save.
 
 local lemma Pr2 &m : 
-Pr [Trapdoor1(P).main() @ &m : res] <=
-Pr [Trapdoor2(P).main() @ &m : res] + Pr[G1(P).main() @ &m : G1.bad]. 
+Pr [Trapdoor1(A).main() @ &m : res] <=
+Pr [Trapdoor2(A).main() @ &m : res] + Pr[G1(A).main() @ &m : M.bad]. 
 proof.
  rewrite (Pr1 &m).
  by apply (Pr2_aux &m).
 save.
 
-local module G2 ( P : Pick) = {
- var bad : bool
- fun main () : bool = {
-  var vX1, vZ1, vX2, vZ2, vY : group;
-  var r, s : gf_q;
-  bad = false;
-  vX1 = $dgroup;
-  r = $dgf_q;
-  s = $dgf_q;
-  vX2 = $dgroup;
-  (vZ1, vZ2, vY) = P.pick(vX1, vX2);
-  if (vZ1 <> (vY^ (log vX1)) /\ ((vZ1 / (vY^ (log vX1))) ^r = (vY^(log vX2)) / vZ2)) {
-   bad = true;
+module G2( A : Adv) ={
+ module TD : O ={
+  fun check (Z1 Z2 Y : group) : bool ={
+  var r : bool = false;
+  if (M.cO < qO /\ ! M.bad){
+   if (Z1 <> (Y^ (log M.gx1)) /\ ((Z1 / (Y^ (log M.gx1))) ^ M.r = (Y^(log M.gx2)) / Z2)) {
+     M.bad = true;
+    }
+    r = ((Z1 / (Y^ (log M.gx1))) ^ M.r = (Y^(log M.gx2)) / Z2);
+   }
+   return r;
   }
-  return ((vZ1 / (vY^ (log vX1))) ^r = (vY^(log vX2)) / vZ2);
+ }
+ module AT = A(TD)
+ fun main () : bool = {
+  var b : bool;
+  M.gx1 = $dgroup;
+  M.r = $dgf_q;
+  M.s = $dgf_q;
+  M.gx2 = $dgroup;
+  M.bad = false; 
+  M.cO = 0;
+  b = AT.run(M.gx1, M.gx2);
+  return b;
  }
 }.
 
+(* local module G2 ( P : Pick) = { *)
+(*  var bad : bool *)
+(*  fun main () : bool = { *)
+(*   var vX1, vZ1, vX2, vZ2, vY : group; *)
+(*   var r, s : gf_q; *)
+(*   bad = false; *)
+(*   vX1 = $dgroup; *)
+(*   r = $dgf_q; *)
+(*   s = $dgf_q; *)
+(*   vX2 = $dgroup; *)
+(*   (vZ1, vZ2, vY) = P.pick(vX1, vX2); *)
+(*   if (vZ1 <> (vY^ (log vX1)) /\ ((vZ1 / (vY^ (log vX1))) ^r = (vY^(log vX2)) / vZ2)) { *)
+(*    bad = true; *)
+(*   } *)
+(*   return ((vZ1 / (vY^ (log vX1))) ^r = (vY^(log vX2)) / vZ2); *)
+(*  } *)
+(*} . *)
+
 local equiv Eq3 : 
-G1(P).main ~ G2(P).main : true ==> G1.bad{1} = G2.bad{2}.
+G1(A).main ~ G2(A).main : true ==> M.bad{1} = M.bad{2}.
 proof.
  fun.
- wp; call (_ : true).
+ wp; call (_ : M.bad, 
+              ={M.gx1, M.gx2, M.r, M.bad, M.cO}, 
+              ={M.bad}).
+ apply run_ll.
+ fun; wp; skip; progress; smt.
+ by intros => ? _; fun; wp; skip; progress; smt.
+ by intros => ?; fun; wp; skip; progress; smt.
  wp.
- rnd (lambda v, g ^ (v - log vX1{2} * r{2}))
-     (lambda u, log u + r{2} * log vX1{2}).
+ rnd (lambda v, g ^ (v - log M.gx1{2} * M.r{2}))
+     (lambda u, log u + M.r{2} * log M.gx1{2}).
  rnd{2}.
- rnd; rnd; wp; skip; progress => //; last 2 by smt.
+ rnd; rnd; wp; skip; progress => //.
  apply lossless. 
  by rewrite mu_x_def_in Dgroup.mu_x_def_in.
  by rewrite supp_def.
  rewrite group_pow_log /Prime_field.(-).
  rewrite -gf_q_add_assoc.
- by rewrite gf_q_mult_comm -(gf_q_add_comm  (rL * log vX1L)) gf_q_add_minus
+ by rewrite gf_q_mult_comm -(gf_q_add_comm  (rL * log gx1L)) gf_q_add_minus
             gf_q_add_comm gf_q_add_unit.
  by rewrite (gf_q_mult_comm rL) /Prime_field.(-) -gf_q_add_assoc gf_q_add_minus
              gf_q_add_comm gf_q_add_unit group_log_pow.
  by rewrite /Cyclic_group_prime.(/) group_pow_log log_pow_mult (gf_q_mult_comm rL).
+ by rewrite /Cyclic_group_prime.(/) group_pow_log log_pow_mult (gf_q_mult_comm rL).
+ smt.
 save. 
 
 local lemma Pr3_aux &m :
-Pr[G1(P).main() @ &m : G1.bad] =
-Pr[G2(P).main() @ &m : G2.bad]. 
+Pr[G1(A).main() @ &m : M.bad] =
+Pr[G2(A).main() @ &m : M.bad]. 
 proof.
  by equiv_deno Eq3.
 save.
 
 local lemma Pr3 &m : 
-Pr [Trapdoor1(P).main() @ &m : res] <=
-Pr [Trapdoor2(P).main() @ &m : res] + Pr[G2(P).main() @ &m : G2.bad]. 
+Pr [Trapdoor1(A).main() @ &m : res] <=
+Pr [Trapdoor2(A).main() @ &m : res] + Pr[G2(A).main() @ &m : M.bad]. 
 proof.
  rewrite -(Pr3_aux &m).
  apply (Pr2 &m).
 save.
-
-local module G3 ( P : Pick) = {
- var bad : bool
- fun main () : bool = {
-  var vX1, vZ1, vX2, vZ2, vY : group;
-  var r, s : gf_q;
-  bad = false;
-  vX1 = $dgroup;
-  vX2 = $dgroup;
-  (vZ1, vZ2, vY) = P.pick(vX1, vX2);
-  if (vZ1 <> (vY^ (log vX1))) {
-   r = $dgf_q;
-   s = $dgf_q;
-   if (((vZ1 / (vY^ (log vX1))) ^r = (vY^(log vX2)) / vZ2)) {
-    bad = true;
-   }
-  }
-  return ((vZ1 / (vY^ (log vX1))) ^r = (vY^(log vX2)) / vZ2);
- }
-}.
-
-
-local equiv Eq4 : 
-G2(P).main ~ G3(P).main : true ==> G2.bad{1} = G3.bad{2}.
-proof.
- fun.
- swap{1} 3 3.
- swap{1} 3 3.
- seq 4 4: (={vX1, vX2, vZ1, vZ2, vY} /\ G2.bad{1} = G3.bad{2}).
- eqobs_in.
- if{2}.
- seq 2 2:
-((={vX1, vX2, vZ1, vZ2, vY, r, s} /\ G2.bad{1} = G3.bad{2}) /\
-  ! vZ1{2} = vY{2} ^ log vX1{2}).
- do 2! rnd; skip; progress => //.
- if{2}.
- rcondt{1} 1.
-  by progress; skip; progress.
-  by wp; skip.
- rcondf{1} 1.
-  progress; skip; smt.
- by skip.
- rcondf{1} 3.
-  by intros => &m; do 2!rnd; skip.
-  do 2! rnd{1}; skip; progress.
-  by apply lossless.
-  by apply lossless.
-save.
-
-local lemma Pr4_aux &m :
-Pr[G2(P).main() @ &m : G2.bad] =
-Pr[G3(P).main() @ &m : G3.bad]. 
-proof.
- by equiv_deno Eq4.
-save.
-
-local lemma Pr4 &m : 
-Pr [Trapdoor1(P).main() @ &m : res] <=
-Pr [Trapdoor2(P).main() @ &m : res] + Pr[G3(P).main() @ &m : G3.bad]. 
-proof.
- rewrite -(Pr4_aux &m).
- apply (Pr3 &m).
-save.
-
-local module G4 ( P : Pick) = {
- var bad : bool
- fun main () : bool = {
-  var vX1, vZ1, vX2, vZ2, vY, z : group;
-  var r, s : gf_q;
-  bad = false;
-  vX1 = $dgroup;
-  vX2 = $dgroup;
-  (vZ1, vZ2, vY) = P.pick(vX1, vX2);
-  if (vZ1 <> (vY^ (log vX1))) {
-   r = $dgf_q;
-   s = $dgf_q;
-   z = $dgroup;
-   if ((z = (vY^(log vX2)) / vZ2)) {
-    bad = true;
-   }
-  }
-  return ((vZ1 / (vY^ (log vX1))) ^r = (vY^(log vX2)) / vZ2);
- }
-}.
-
-require import Distr.
-
-
-lemma log_inj : forall X Y, log X = log Y => X = Y.
-proof.
- intros => X Y.
- cut:= gen_def X => [[x]] ->.
- cut:= gen_def Y => [[y]] ->.
- by rewrite !group_pow_log => ->.
-save.
-
-local equiv Eq5 : 
-G3(P).main ~ G4(P).main : true ==> G3.bad{1} = G4.bad{2}.
-proof.
- fun.
- seq 4 4: (={vX1, vX2, vZ1, vZ2, vY} /\ G3.bad{1} = G4.bad{2}).
-  eqobs_in.
- if => //.
- seq 2 3: 
- (={vX1, vX2, vZ1, vZ2, vY} /\ G3.bad{1} = G4.bad{2} /\
-  ! vZ1{1} = vY{1} ^ log vX1{1} /\ z{2} = (vZ1 / vY ^ log vX1){1} ^ r{1}).
- swap{2} 3 -1.
- rnd.
- rnd (lambda v, (vZ1 / vY ^ log vX1){2} ^ v)
-     (lambda v, log v / ((log vZ1 - log ( vY ^ log vX1))){2}).
- rnd{2}.
- wp; skip.
- progress => //.
- apply lossless.
- by rewrite mu_x_def_in Dgroup.mu_x_def_in.
- by apply supp_def.
- rewrite  /Cyclic_group_prime.(/).
- rewrite log_pow_mult group_pow_log.
- rewrite /Prime_field.(/).
- rewrite -gf_q_mult_assoc.
- rewrite gf_q_mult_inv.
- cut: log vZ1{2} - log (vY{2} ^ log vX1{2}) = gf_q0 => vZ1{2} = vY{2} ^ log vX1{2}; last smt. 
- intros  => heq.
- cut := neg_zero (log vZ1{2}) (log (vY{2} ^ log vX1{2})) _.
-  by rewrite heq.
- intros => {heq} heq.
- by apply log_inj.
- by rewrite gf_q_mult_unit.
- rewrite  /Cyclic_group_prime.(/) group_pow_mult.
- rewrite /Prime_field.(/).
- rewrite gf_q_mult_assoc. 
- rewrite gf_q_mult_comm. 
- rewrite gf_q_mult_assoc.
- rewrite (gf_q_mult_comm (inv (log vZ1{2} - log (vY{2} ^ log vX1{2})))).  
- rewrite gf_q_mult_inv.
- cut: log vZ1{2} - log (vY{2} ^ log vX1{2}) = gf_q0 => vZ1{2} = vY{2} ^ log vX1{2}; last smt. 
- intros  => heq.
- cut := neg_zero (log vZ1{2}) (log (vY{2} ^ log vX1{2})) _.
-  by rewrite heq.
- intros => {heq} heq.
- by apply log_inj.
- rewrite gf_q_mult_comm gf_q_mult_unit.
- by rewrite group_log_pow.
- if.
- progress => //. 
- wp; skip; progress.
- wp; skip; progress.
-save.
-
-local lemma Pr5_aux &m :
-Pr[G3(P).main() @ &m : G3.bad] =
-Pr[G4(P).main() @ &m : G4.bad]. 
-proof.
- by equiv_deno Eq5.
-save.
-
-local lemma Pr5 &m : 
-Pr [Trapdoor1(P).main() @ &m : res] <=
-Pr [Trapdoor2(P).main() @ &m : res] + Pr[G4(P).main() @ &m : G4.bad]. 
-proof.
- rewrite -(Pr5_aux &m).
- apply (Pr4 &m).
-save.
-
-
-local module G5 ( P : Pick) = {
- fun main () : bool = {
-  var vX1, vZ1, vX2, vZ2, vY, z : group;
-  var r, s : gf_q;
-  vX1 = $dgroup;
-  vX2 = $dgroup;
-  (vZ1, vZ2, vY) = P.pick(vX1, vX2);
-  z = $dgroup;
-  return ((z = (vY^(log vX2)) / vZ2));
- }
-}.
-
-
-local equiv Eq6 : 
-G4(P).main ~ G5(P).main : true ==> G4.bad{1} => res{2}.
-proof.
- fun.
- seq 4 3: (={vX1, vX2, vZ1, vZ2, vY} /\ G4.bad{1} = false).
- by call (_ : true); do 2! rnd; wp; skip; progress.
- if{1} => //; last by rnd{2}; skip; progress; apply Dgroup.lossless.
- wp; rnd; do 2! rnd{1}; skip; progress => //.
- apply lossless.
-save.
-
-local lemma Pr6_aux &m :
-Pr[G4(P).main() @ &m : G4.bad] <=
-Pr[G5(P).main() @ &m : res]. 
-proof.
- by equiv_deno Eq6.
-save.
-
-local lemma Pr6_aux2 &m : Pr [G5(P).main() @ &m : res] = 1%r / q%r.
-proof.
- bdhoare_deno (_ : true ==> res).
- fun.
- rnd.
- call (_ : true).
- apply pick_ll.
- do 2! rnd; skip; progress => //.
- cut -> : ((lambda (x : group),
-     forall (result : group * group * group),
-       let (vZ1, vZ2, vY) = result in
-       mu dgroup (lambda (x0 : group), x0 = vY ^ log x / vZ2) = 1%r / q%r) = cpTrue).
- apply fun_ext; rewrite /Fun.(==) /cpTrue /=.
- progress.
- apply (_ : forall p, p => p = true);first smt.
- progress => //.
-  rewrite -(Dgroup.mu_x_def_in ( x3 ^ log x / x2)) .
-  rewrite /mu_x.
-  apply Distr.mu_eq.
-  rewrite /Fun.(==) => /= x'.
-  smt.
-  by rewrite -Dgroup.lossless /weight.
-  by rewrite -Dgroup.lossless /weight.
-  trivial.
-  trivial.
-save.
-
-lemma Conclusion &m : 
-Pr [Trapdoor1(P).main() @ &m : res] <=
-Pr [Trapdoor2(P).main() @ &m : res] + 1%r / q%r. 
-proof.
- rewrite -(Pr6_aux2 &m).
- apply (Real.Trans _ 
-     (Pr[Trapdoor2(P).main() @ &m : res] + Pr[G4(P).main() @ &m : G4.bad]) _).
- apply (Pr5 &m).
- cut := Pr6_aux &m.
- smt.
-save.
-
-end section.
